Move from small-step to a big-step semantics
Rename "standard_result" to "stmt_result_total"
Move unused files to "archive"

ExpProofGenTest.thy
@@ -28,41 +28,54 @@ definition assert_rel :: "('a full_total_state \<Rightarrow> ('a vbpl_absval) ns
 
 text\<open> Points to think about:
   \<^item> backward vs. forward simulation (also tracking single Boogie state vs sets of Boogie states)
-  \<^item> small-step vs big-step semantics
-  \<^item> current version is non-compositional, since it does not give information to what the Boogie reduction
-    reduces (generalization is not straightforward here, because of the Viper small-step reduction)
 \<close>
 
-definition stmt_rel_simple :: "('a full_total_state \<Rightarrow> ('a vbpl_absval) nstate \<Rightarrow> bool) \<Rightarrow>
+definition stmt_rel :: "('a full_total_state \<Rightarrow> ('a vbpl_absval) nstate \<Rightarrow> bool) \<Rightarrow>
                                ('a full_total_state \<Rightarrow> ('a vbpl_absval) nstate \<Rightarrow> bool) \<Rightarrow> 
                                 'a total_context \<Rightarrow> ('a full_total_state \<Rightarrow> bool) \<Rightarrow> 
                                 type_context \<Rightarrow> 'a astcontext_bpl \<Rightarrow>
-                                ViperLang.stmt \<Rightarrow> (Ast.bigblock \<times> cont) \<Rightarrow> bool"
+                                ViperLang.stmt \<Rightarrow> (Ast.bigblock \<times> cont) \<Rightarrow> (Ast.bigblock \<times> cont) \<Rightarrow> bool"
   where 
-    "stmt_rel_simple R R' ctxt_vpr StateCons \<Lambda> ctxt stmt_vpr \<gamma> \<equiv>
-      \<forall> \<omega> ns stmt'_vpr res. R \<omega> ns \<longrightarrow> 
-             red_stmt_total_multi ctxt_vpr StateCons \<Lambda> (Inl stmt_vpr, RNormal \<omega>) (stmt'_vpr, res) \<longrightarrow>
+    "stmt_rel R R' ctxt_vpr StateCons \<Lambda> ctxt stmt_vpr \<gamma> \<gamma>' \<equiv>
+      \<forall> \<omega> ns res. R \<omega> ns \<longrightarrow> 
+             red_stmt_total ctxt_vpr StateCons \<Lambda> stmt_vpr \<omega> res \<longrightarrow>
              (\<forall>\<omega>'. res = RNormal \<omega>' \<longrightarrow>
-                 \<comment>\<open>Since the target configuration \<gamma>' is existentially quantified, we cannot connect
-                    this result to a subsequent Boogie statement.\<close> 
-                 (\<exists>\<gamma>' ns'. red_ast_bpl ctxt (\<gamma>, Normal ns) (\<gamma>', Normal ns') \<and> R' \<omega>' ns')) \<and>
+                 (\<exists>ns'. (red_ast_bpl ctxt (\<gamma>, Normal ns) (\<gamma>', Normal ns') \<and> R' \<omega>' ns'))) \<and>
              (res = RFailure \<longrightarrow> 
-                (\<exists>c'.  snd c' = Failure \<and>
+                (\<exists>c'. snd c' = Failure \<and>
                       red_ast_bpl ctxt (\<gamma>, Normal ns) c'))"
 
-lemma stmt_rel_simple_intro[case_names base step]:
+lemma stmt_rel_intro[case_names base step]:
   assumes 
-  "\<And>\<omega> ns stmt'_vpr \<omega>' res. 
+  "\<And>\<omega> ns \<omega>'. 
           R \<omega> ns \<Longrightarrow> 
-          red_stmt_total_multi Pr \<Lambda> ctxt_vpr (Inl stmt_vpr, RNormal \<omega>) (stmt'_vpr, RNormal \<omega>') \<Longrightarrow>
-          \<exists>\<gamma>' ns'. red_ast_bpl ctxt (\<gamma>, Normal ns) (\<gamma>', Normal ns') \<and> R' \<omega>' ns'" and
-  "\<And>\<omega> ns stmt'_vpr res.
+          red_stmt_total ctxt_vpr StateCons \<Lambda> stmt_vpr \<omega> (RNormal \<omega>') \<Longrightarrow>
+          \<exists>ns'. (red_ast_bpl ctxt (\<gamma>, Normal ns) (\<gamma>', Normal ns') \<and> R' \<omega>' ns')" and
+  "\<And>\<omega> ns.
           R \<omega> ns \<Longrightarrow> 
-          red_stmt_total_multi Pr \<Lambda> ctxt_vpr (Inl stmt_vpr, RNormal \<omega>) (stmt'_vpr, RFailure) \<Longrightarrow>
+          red_stmt_total ctxt_vpr StateCons \<Lambda> stmt_vpr \<omega> RFailure \<Longrightarrow>
           \<exists>c'. snd c' = Failure \<and> red_ast_bpl ctxt (\<gamma>, Normal ns) c'"
-  shows "stmt_rel_simple R R' Pr \<Lambda> ctxt_vpr ctxt stmt_vpr \<gamma>"
+  shows "stmt_rel R R' ctxt_vpr StateCons \<Lambda> ctxt stmt_vpr \<gamma> \<gamma>'"
   using assms
-  unfolding stmt_rel_simple_def
+  unfolding stmt_rel_def  
+  by blast
+
+lemma stmt_rel_normal_elim:
+  assumes "stmt_rel R R' ctxt_vpr StateCons \<Lambda> ctxt stmt_vpr \<gamma> \<gamma>'" and
+          "R \<omega> ns" and
+          "red_stmt_total ctxt_vpr StateCons \<Lambda> stmt_vpr \<omega> (RNormal \<omega>')"
+    shows   "\<exists>ns'. (red_ast_bpl ctxt (\<gamma>, Normal ns) (\<gamma>', Normal ns') \<and> R' \<omega>' ns')"
+  using assms
+  unfolding stmt_rel_def
+  by blast
+
+lemma stmt_rel_failure_elim:
+  assumes "stmt_rel R R' ctxt_vpr StateCons \<Lambda> ctxt stmt_vpr \<gamma> \<gamma>'" and
+          "R \<omega> ns" and
+          "red_stmt_total ctxt_vpr StateCons \<Lambda> stmt_vpr \<omega> RFailure"
+  shows "\<exists>c'. snd c' = Failure \<and> red_ast_bpl ctxt (\<gamma>, Normal ns) c'"
+  using assms
+  unfolding stmt_rel_def
   by blast
 
 definition type_interp_rel_wf :: "('a \<Rightarrow> abs_type) \<Rightarrow> ('a vbpl_absval) absval_ty_fun  \<Rightarrow> 'a ty_repr_bpl \<Rightarrow> bool"
@@ -132,36 +145,21 @@ lemma assign_rel_simple:
   and
           ExpRel: "exp_rel_vpr_bpl R3 ctxt_vpr (econtext_bpl.truncate ctxt) e_vpr e_bpl" 
           
-  shows "stmt_rel_simple R2 R2 ctxt_vpr StateCons \<Lambda>_vpr ctxt (ViperLang.LocalAssign x_vpr e_vpr) \<gamma>"  
-proof (cases rule: stmt_rel_simple_intro)
+        shows "stmt_rel R2 R2 ctxt_vpr StateCons \<Lambda>_vpr ctxt (ViperLang.LocalAssign x_vpr e_vpr) 
+               \<gamma>
+               (BigBlock name cs str tr, cont)" (is "stmt_rel R2 R2 ctxt_vpr StateCons \<Lambda>_vpr ctxt (ViperLang.LocalAssign x_vpr e_vpr) \<gamma> ?\<gamma>'") 
+proof (cases rule: stmt_rel_intro)
 \<comment>\<open>normal case\<close>
-  fix \<omega> ns stmt'_vpr \<omega>' res
-  assume R: "R2 \<omega> ns" and    
-         RedVpr: "red_stmt_total_multi ctxt_vpr StateCons \<Lambda>_vpr (Inl (LocalAssign x_vpr e_vpr), RNormal \<omega>) (stmt'_vpr, RNormal \<omega>')"
+  fix \<omega> ns \<omega>'
+  assume R: "R2 \<omega> ns" and
+         RedVpr: "red_stmt_total ctxt_vpr StateCons \<Lambda>_vpr (LocalAssign x_vpr e_vpr) \<omega> (RNormal \<omega>')"
 
-  from RedVpr
-  show "\<exists>\<gamma>' ns'. red_ast_bpl ctxt (\<gamma>, Normal ns) (\<gamma>', Normal ns') \<and> R2 \<omega>' ns'"
-  proof (cases rule: converse_rtranclpE)
-    case base
-    hence "\<omega>' = \<omega>"
-      by auto
-    show ?thesis
-      apply (rule exI)
-      apply (rule exI[where ?x=ns])
-      by (auto simp: \<open>\<omega>' = \<omega>\<close> R)
-  next
-    case (step y)    
-    from this obtain stmt''_vpr \<omega>'' where "y = (stmt''_vpr, RNormal \<omega>'')"
-      using red_stmt_total_multi_normal_source
-      by (metis snd_conv surjective_pairing)
-
-    from step(1) obtain v where RedEVpr: "ctxt_vpr, StateCons, (Some \<omega>) \<turnstile> \<langle>e_vpr; \<omega>\<rangle> [\<Down>]\<^sub>t (Val v)" and 
-                                yEq: "y = (Inr (), RNormal (update_var_total \<omega> x_vpr v))" and
-                                "\<omega>'' = (update_var_total \<omega> x_vpr v)" and
-                                vTyVpr: "get_type (absval_interp_total ctxt_vpr) v = ty"
-      apply (rule NormalSingleStep_case)
-      apply (simp only: \<open>y = _\<close>)
-      apply (rule red_stmt_total_single_set.cases)
+  show "\<exists>ns'. red_ast_bpl ctxt (\<gamma>, Normal ns) (?\<gamma>', Normal ns') \<and> R2 \<omega>' ns'"
+  proof -
+    from RedVpr obtain v where RedEVpr: "ctxt_vpr, StateCons, (Some \<omega>) \<turnstile> \<langle>e_vpr; \<omega>\<rangle> [\<Down>]\<^sub>t (Val v)" and 
+                                "\<omega>' = (update_var_total \<omega> x_vpr v)" and
+                                vTyVpr: "get_type (absval_interp_total ctxt_vpr) v = ty"      
+      apply (rule red_stmt_total.cases)
       using VprTy
       by auto
 
@@ -172,7 +170,6 @@ proof (cases rule: stmt_rel_simple_intro)
       by blast
 
     let ?v_bpl = "val_rel_vpr_bpl v"
-    let ?ns'' = "update_var (var_context ctxt) ns' x_bpl ?v_bpl"
     have RedEBpl:"red_expr_bpl (econtext_bpl.truncate ctxt) e_bpl ns' ?v_bpl"
       apply (rule exp_rel_vpr_bpl_elim_2[OF ExpRel])
       using R' RedEVpr R_def
@@ -183,7 +180,9 @@ proof (cases rule: stmt_rel_simple_intro)
       unfolding type_interp_rel_wf_def
       by simp
 
-    have "red_ast_bpl ctxt ((?b, cont), Normal ns') ((BigBlock name cs str tr, cont), Normal ?ns'')"
+    let ?ns'' = "update_var (var_context ctxt) ns' x_bpl ?v_bpl"
+
+    have RedBpl: "red_ast_bpl ctxt ((?b, cont), Normal ns') ((BigBlock name cs str tr, cont), Normal ?ns'')"
       apply (rule converse_rtranclp_into_rtranclp)
        apply rule
        apply rule
@@ -192,60 +191,36 @@ proof (cases rule: stmt_rel_simple_intro)
       using RedEBpl
       by auto
 
-    have "R3 \<omega>'' \<omega>'' ?ns''" 
-      apply (subst \<open>\<omega>'' = _\<close>)+
+    moreover have "R3 \<omega>' \<omega>' ?ns''" 
+      apply (subst \<open>\<omega>' = _\<close>)+
       using R_def RAssign R' vTyVpr ValBplTy 
       by auto
 
-    moreover from step(2) have "\<omega>' = (update_var_total \<omega> x_vpr v)"
-      apply (subst (asm) yEq)
-      using red_stmt_total_multi_final
-      by blast
-
     ultimately show ?thesis 
-      using RedBplWf R_def
-      apply (simp only: \<open>\<omega>'' = _\<close>)
-      by (meson \<open>red_ast_bpl ctxt ((BigBlock name (Assign x_bpl e_bpl # cs) str tr, cont), Normal ns') ((BigBlock name cs str tr, cont), Normal (update_var (econtext_bpl.var_context ctxt) ns' x_bpl (val_rel_vpr_bpl v)))\<close> rtranclp_trans)
+      using RedBplWf R_def \<open>\<omega>' = _\<close>
+      by (meson rtranclp_trans)
   qed
 next
   \<comment>\<open>Failure case\<close>
-  fix \<omega> ns stmt'_vpr res
+  fix \<omega> ns 
   assume "R2 \<omega> ns" and 
-         RedVpr:"red_stmt_total_multi ctxt_vpr StateCons \<Lambda>_vpr (Inl (LocalAssign x_vpr e_vpr), RNormal \<omega>) (stmt'_vpr, RFailure)"
+         RedVpr:"red_stmt_total ctxt_vpr StateCons \<Lambda>_vpr (LocalAssign x_vpr e_vpr) \<omega> RFailure"
   
   from RedVpr show "\<exists>c'. snd c' = Failure \<and> red_ast_bpl ctxt (\<gamma>, Normal ns) c'"
-  proof (cases rule: converse_rtranclpE)
-    case base
-    then show ?thesis by simp
-  next
-    case (step y)
-    from step(1)
-    show "\<exists>c'. snd c' = Failure \<and> red_ast_bpl ctxt (\<gamma>, Normal ns) c'"
-    proof cases
-      case NormalSingleStep
-      then show ?thesis 
-      proof cases
-        case (RedLocalAssign v ty)        
-        then show ?thesis using red_stmt_total_multi_final step
-          by blast
-      next 
-        case (RedSubExpressionFailure e)
-        hence "ctxt_vpr, StateCons, Some \<omega> \<turnstile> \<langle>e_vpr;\<omega>\<rangle> [\<Down>]\<^sub>t VFailure"
-          by simp
+  proof cases
+  case (RedSubExpressionFailure e)
+  hence "ctxt_vpr, StateCons, Some \<omega> \<turnstile> \<langle>e_vpr;\<omega>\<rangle> [\<Down>]\<^sub>t VFailure"
+    by simp
 
-        then show ?thesis 
-          using  R_def \<open>R2 \<omega> ns\<close> wf_rel_failure_elim[OF ExpWfRel]
-          by blast
-      qed
-    qed
+  then show ?thesis 
+    using  R_def \<open>R2 \<omega> ns\<close> wf_rel_failure_elim[OF ExpWfRel]
+    by blast
   qed
 qed
 
 text \<open>Relational rule for Viper assignment \<open>x := e_vpr\<close>\<close>
 lemma assign_rel_simple_2:
-  assumes R_def: (*"R2 = (\<lambda> \<omega> ns. state_rel Pr Trep Tr (econtext_bpl.truncate ctxt) (mask_var Tr) \<omega> \<omega> ns)"
-                     "R3 = (\<lambda> \<omega>def \<omega> ns. \<omega>def = \<omega> \<and> state_rel Pr Trep Tr (econtext_bpl.truncate ctxt) (mask_var Tr) \<omega> \<omega> ns)"*)
-                   "R3 = (\<lambda> \<omega>def \<omega> ns. \<omega>def = \<omega> \<and> R2 \<omega> ns)" and
+  assumes R_def: "R3 = (\<lambda> \<omega>def \<omega> ns. \<omega>def = \<omega> \<and> R2 \<omega> ns)" and
           VprTy: "\<Lambda>_vpr x_vpr = Some ty" and
           ExpWfRel: "expr_wf_rel R3 ctxt_vpr StateCons ctxt e_vpr \<gamma> \<gamma>'" and
           ProgressToAssign: "\<And>\<omega>_def \<omega> ns2. R3 \<omega>_def \<omega> ns2 \<Longrightarrow> 
@@ -262,7 +237,9 @@ lemma assign_rel_simple_2:
   and
           ExpRel: "exp_rel_vpr_bpl R3 ctxt_vpr (econtext_bpl.truncate ctxt) e_vpr e_bpl" 
           
-        shows "stmt_rel_simple R2 R2 ctxt_vpr StateCons \<Lambda>_vpr ctxt (ViperLang.LocalAssign x_vpr e_vpr) \<gamma>"  
+        shows "stmt_rel R2 R2 ctxt_vpr StateCons \<Lambda>_vpr ctxt (ViperLang.LocalAssign x_vpr e_vpr) 
+               \<gamma>
+               (BigBlock name cs str tr, cont)"
 proof -  
   from ExpWfRel and ProgressToAssign 
   have *:"expr_wf_rel R3 ctxt_vpr StateCons ctxt e_vpr \<gamma> ((BigBlock name ((Lang.Assign x_bpl e_bpl)#cs) str tr), cont)"
@@ -275,9 +252,33 @@ proof -
 qed
 
 lemma stmt_rel_simple_propagate:
-  assumes "\<And> \<omega> ns. R \<omega> ns \<Longrightarrow> \<exists>ns'. red_ast_bpl ctxt (\<gamma>, Normal ns) (\<gamma>', Normal ns') \<and> R'' \<omega> ns'" and
-          "stmt_rel_simple R'' R' Pr ctxt_vpr \<Lambda>_vpr ctxt stmt_vpr \<gamma>'"
-  shows "stmt_rel_simple R R' Pr ctxt_vpr \<Lambda>_vpr ctxt stmt_vpr \<gamma>"
-  sorry
+  assumes "\<And> \<omega> ns. R0 \<omega> ns \<Longrightarrow> \<exists>ns'. red_ast_bpl ctxt (\<gamma>0, Normal ns) (\<gamma>1, Normal ns') \<and> R1 \<omega> ns'" and
+          "stmt_rel R1 R2 ctxt_vpr StateCons \<Lambda>_vpr ctxt stmt_vpr \<gamma>1 \<gamma>2"
+        shows "stmt_rel R0 R2 ctxt_vpr StateCons \<Lambda>_vpr ctxt stmt_vpr \<gamma>0 \<gamma>2"  
+proof (rule stmt_rel_intro)
+  fix \<omega> ns \<omega>'
+  assume "R0 \<omega> ns" and
+         RedVpr: "red_stmt_total ctxt_vpr StateCons \<Lambda>_vpr stmt_vpr \<omega> (RNormal \<omega>')"
+
+  from \<open>R0 \<omega> ns\<close> and assms(1) obtain ns1 where
+    "red_ast_bpl ctxt (\<gamma>0, Normal ns) (\<gamma>1, Normal ns1)" and "R1 \<omega> ns1"
+    by blast
+
+  thus "\<exists>ns'. red_ast_bpl ctxt (\<gamma>0, Normal ns) (\<gamma>2, Normal ns') \<and> R2 \<omega>' ns'"
+    using stmt_rel_normal_elim[OF assms(2)] RedVpr
+    by (meson rtranclp_trans)
+next
+  fix \<omega> ns \<omega>'
+  assume "R0 \<omega> ns" and
+         RedVpr: "red_stmt_total ctxt_vpr StateCons \<Lambda>_vpr stmt_vpr \<omega> RFailure"
+
+  from \<open>R0 \<omega> ns\<close> and assms(1) obtain ns1 where
+    "red_ast_bpl ctxt (\<gamma>0, Normal ns) (\<gamma>1, Normal ns1)" and "R1 \<omega> ns1"
+    by blast
+
+  thus "\<exists>c'. snd c' = Failure \<and> red_ast_bpl ctxt (\<gamma>0, Normal ns) c'"
+    using stmt_rel_failure_elim[OF assms(2)] RedVpr
+    by (meson rtranclp_trans)
+qed
 
 end
