TotalSemantics.thy
@@ -118,7 +118,7 @@ lemma exhale_state_same_store: "\<omega>' \<in> exhale_state \<omega> m \<Longri
 lemma exhale_state_same_trace: "\<omega>' \<in> exhale_state \<omega> m \<Longrightarrow> get_trace_total \<omega>' = get_trace_total \<omega>"
   by (simp add: exhale_state_def)
 
-inductive fold_rel :: "'a total_context \<Rightarrow> ('a full_total_state \<Rightarrow> bool) \<Rightarrow> predicate_ident \<Rightarrow> ('a val list) \<Rightarrow> prat \<Rightarrow> 'a full_total_state \<Rightarrow> 'a standard_result \<Rightarrow> bool"
+inductive fold_rel :: "'a total_context \<Rightarrow> ('a full_total_state \<Rightarrow> bool) \<Rightarrow> predicate_ident \<Rightarrow> ('a val list) \<Rightarrow> prat \<Rightarrow> 'a full_total_state \<Rightarrow> 'a stmt_result_total \<Rightarrow> bool"
   where 
     FoldRelNormal: 
       "\<lbrakk> ViperLang.predicates (program_total ctxt) pred_id = Some pred_decl;
@@ -144,31 +144,29 @@ fun sub_expressions :: "stmt \<Rightarrow> pure_exp set" where
 | "sub_expressions _ = {}"
 \<comment>\<open>TODO: \<^const>\<open>sub_expressions\<close> is duplicated from ViperLang\<close>
 
-inductive red_stmt_total_single_set :: "'a total_context \<Rightarrow> ('a full_total_state \<Rightarrow> bool) \<Rightarrow> type_context \<Rightarrow>  stmt \<Rightarrow> 'a full_total_state  \<Rightarrow> (stmt+unit) \<times> ('a standard_result) \<Rightarrow> bool"
+inductive red_stmt_total :: "'a total_context \<Rightarrow> ('a full_total_state \<Rightarrow> bool) \<Rightarrow> type_context \<Rightarrow> stmt \<Rightarrow> 'a full_total_state  \<Rightarrow> 'a stmt_result_total \<Rightarrow> bool"
   for ctxt :: "'a total_context" and R :: "('a full_total_state \<Rightarrow> bool)" and \<Lambda> :: "type_context"  where
 \<comment>\<open>Atomic statements\<close>
-   RedSkip: "red_stmt_total_single_set ctxt R \<Lambda> Skip \<omega> (Inr (), RNormal \<omega>)" 
+   RedSkip: "red_stmt_total ctxt R \<Lambda> Skip \<omega> (RNormal \<omega>)" 
  | RedInhale: 
    "\<lbrakk> red_inhale ctxt R A \<omega> res \<rbrakk> \<Longrightarrow>
-      red_stmt_total_single_set ctxt R \<Lambda> (Inhale A) \<omega> (Inr (), res)"
+      red_stmt_total ctxt R \<Lambda> (Inhale A) \<omega> res"
  | RedExhale:
    "\<lbrakk> red_exhale ctxt R \<omega> A (get_m_total_full \<omega>) (ExhaleNormal m');
       \<omega>' \<in> exhale_state \<omega> m' \<rbrakk> \<Longrightarrow>
-      red_stmt_total_single_set ctxt R \<Lambda> (Exhale A) \<omega> (Inr (), RNormal \<omega>')"
+      red_stmt_total ctxt R \<Lambda> (Exhale A) \<omega> (RNormal \<omega>')"
  | RedExhaleFailure:
    "\<lbrakk> red_exhale ctxt R \<omega> A (get_m_total_full \<omega>) ExhaleFailure \<rbrakk> \<Longrightarrow>
-      red_stmt_total_single_set ctxt R \<Lambda> (Exhale A) \<omega> (Inr (), RFailure)"
+      red_stmt_total ctxt R \<Lambda> (Exhale A) \<omega> RFailure"
  | RedAssert:
    "\<lbrakk> red_exhale ctxt R \<omega> A (get_m_total_full \<omega>) (ExhaleNormal m') \<rbrakk> \<Longrightarrow>
-      red_stmt_total_single_set ctxt R \<Lambda> (Assert A) \<omega> (Inr (), RNormal \<omega>)"
+      red_stmt_total ctxt R \<Lambda> (Assert A) \<omega> (RNormal \<omega>)"
  | RedAssertFailure:
    "\<lbrakk> red_exhale ctxt R \<omega> A (get_m_total_full \<omega>) ExhaleFailure \<rbrakk> \<Longrightarrow>
-      red_stmt_total_single_set ctxt R \<Lambda> (Assert A) \<omega> (Inr (), RFailure)"
+      red_stmt_total ctxt R \<Lambda> (Assert A) \<omega> RFailure"
 
 \<comment>\<open>Note that exhale is demonic here (even locally). For instance, exhale acc(x.f, wildcard) * acc(x.f, 1/2)
-always has at least one failure transition, which is not in-sync with Carbon's reordering heuristic for
-wildcards. We might want to make exhale locally angelic instead. The premise in Failure rule would have to 
-be changed to\<^term>\<open>\<forall>res. red_exhale Pr ctxt \<omega> A (get_m_total_full \<omega>) res \<longrightarrow> res = ExhaleFailure\<close>\<close>
+always has at least one failure transition. This is in-sync with the recent Carbon upgrade.\<close>
 
 
 \<comment>\<open>TODO: Add semantics for \<^term>\<open>Assume A\<close>. \<close>
@@ -178,35 +176,34 @@ be changed to\<^term>\<open>\<forall>res. red_exhale Pr ctxt \<omega> A (get_m_t
    "\<lbrakk> ctxt, R, (Some \<omega>) \<turnstile> \<langle>e; \<omega>\<rangle> [\<Down>]\<^sub>t (Val v);
       \<Lambda> x = Some ty; 
       get_type (absval_interp_total ctxt) v = ty \<rbrakk> \<Longrightarrow> 
-     red_stmt_total_single_set ctxt R \<Lambda> (LocalAssign x e) \<omega> (Inr (), (RNormal (update_var_total \<omega> x v)))"
+     red_stmt_total ctxt R \<Lambda> (LocalAssign x e) \<omega> (RNormal (update_var_total \<omega> x v))"
  | RedFieldAssign: 
    "\<lbrakk> ctxt, R, (Some \<omega>) \<turnstile> \<langle>e_r; \<omega>\<rangle> [\<Down>]\<^sub>t Val (VRef (Address addr));
       get_mh_total_full \<omega> (addr,f) = pwrite;
       ctxt, R, (Some \<omega>)  \<turnstile> \<langle>e; \<omega>\<rangle> [\<Down>]\<^sub>t Val v \<rbrakk> \<Longrightarrow> 
-      red_stmt_total_single_set ctxt R \<Lambda> (FieldAssign e_r f e) \<omega> (Inr (), (RNormal (update_hh_loc_total_full \<omega> (addr,f) v)))"
+      red_stmt_total ctxt R \<Lambda> (FieldAssign e_r f e) \<omega> (RNormal (update_hh_loc_total_full \<omega> (addr,f) v))"
 \<comment>\<open>Is null case handled in NestedPermSem?\<close>
  | RedFieldAssignFailure: 
    "\<lbrakk> ctxt, R, (Some \<omega>) \<turnstile> \<langle>e_r; \<omega>\<rangle> [\<Down>]\<^sub>t Val (VRef r);
       r = Null \<or> get_mh_total_full \<omega> (the_address r,f) \<noteq> pwrite \<rbrakk> \<Longrightarrow> 
-      red_stmt_total_single_set ctxt R \<Lambda> (FieldAssign e_r f e) \<omega> (Inr (), (RNormal (update_hh_loc_total_full \<omega> (addr,f) v)))"
+      red_stmt_total ctxt R \<Lambda> (FieldAssign e_r f e) \<omega> (RNormal (update_hh_loc_total_full \<omega> (addr,f) v))"
 
 | RedUnfold:
   "\<lbrakk> red_pure_exps_total ctxt R (Some \<omega>) e_args \<omega> (Some v_args);
      ctxt, R, (Some \<omega>) \<turnstile> \<langle>e_p; \<omega>\<rangle> [\<Down>]\<^sub>t Val (VPerm v_p);     
      W' = {\<omega>2. unfold_rel ctxt R pred_id v_args (Abs_prat v_p) \<omega> \<omega>2 \<and> total_heap_consistent ctxt \<omega>2};
      th_result_rel (v_p > 0 \<and> v_p \<le> Rep_prat (get_mp_total_full \<omega> (pred_id, v_args))) True W' res \<rbrakk> \<Longrightarrow>
-    red_stmt_total_single_set ctxt R \<Lambda> (Unfold pred_id e_args (PureExp e_p)) \<omega> (Inr (), res)"
+    red_stmt_total ctxt R \<Lambda> (Unfold pred_id e_args (PureExp e_p)) \<omega> res"
 
 \<comment>\<open>\<^const>\<open>unfold_rel\<close> constrains permission \<^term>\<open>p\<close> to be strictly positive\<close>
 | RedUnfoldWildcard:
   "\<lbrakk> red_pure_exps_total ctxt R (Some \<omega>) e_args \<omega> (Some v_args);
      unfold_rel ctxt R pred_id v_args p \<omega> \<omega>' \<rbrakk> \<Longrightarrow>
-    red_stmt_total_single_set ctxt R \<Lambda> (Unfold pred_id e_args Wildcard) \<omega> (Inr (), RNormal \<omega>')"
+    red_stmt_total ctxt R \<Lambda> (Unfold pred_id e_args Wildcard) \<omega> (RNormal \<omega>')"
 | RedUnfoldWildcardFailure:
   "\<lbrakk> red_pure_exps_total ctxt R (Some \<omega>) e_args \<omega> (Some v_args);
      get_mp_total_full \<omega> (pred_id, v_args) = pnone \<rbrakk> \<Longrightarrow>
-    red_stmt_total_single_set ctxt R \<Lambda> (Unfold pred_id e_args Wildcard) \<omega> 
-      (Inr (), RFailure)"
+    red_stmt_total ctxt R \<Lambda> (Unfold pred_id e_args Wildcard) \<omega> RFailure"
 \<comment>\<open>TODO: unfold acc(P(x),0)\<close>
 
 \<comment>\<open>One should be able to prove that if \<omega> is unfolding consistent, then so is \<omega>' after a fold, without
@@ -218,60 +215,45 @@ be changed to\<^term>\<open>\<forall>res. red_exhale Pr ctxt \<omega> A (get_m_t
      ctxt, R, (Some \<omega>) \<turnstile> \<langle>e_p; \<omega>\<rangle> [\<Down>]\<^sub>t Val (VPerm v_p);     
      fold_rel ctxt R pred_id v_args (Abs_prat v_p) \<omega> res
  \<rbrakk> \<Longrightarrow>
-    red_stmt_total_single_set ctxt R \<Lambda> (Fold pred_id e_args (PureExp e_p)) \<omega> (Inr (), res)"
+    red_stmt_total ctxt R \<Lambda> (Fold pred_id e_args (PureExp e_p)) \<omega> res"
 
 | RedFoldWildcard:
   "\<lbrakk> red_pure_exps_total ctxt R (Some \<omega>) e_args \<omega> (Some v_args);     
      fold_rel ctxt R pred_id v_args p \<omega> res \<rbrakk> \<Longrightarrow>
-    red_stmt_total_single_set ctxt R \<Lambda> (Fold pred_id e_args Wildcard) \<omega> (Inr (), res)"
+    red_stmt_total ctxt R \<Lambda> (Fold pred_id e_args Wildcard) \<omega> res"
 \<comment>\<open>TODO: fold acc(P(x),0)\<close>
 
 \<comment>\<open>Composite statements\<close>
+| RedScope:
+    "\<lbrakk>  v \<in> set_from_type (absval_interp_total ctxt) \<tau>;
+       red_stmt_total ctxt R \<Lambda> scopeBody (shift_and_add_state \<omega> v) res;
+       res_unshift = map_stmt_result_total (unshift_state 0) res \<rbrakk> \<Longrightarrow>
 
+      red_stmt_total ctxt R \<Lambda> (Scope \<tau> scopeBody) \<omega> res_unshift"
  | RedIfTrue: 
    "\<lbrakk> ctxt, R, (Some \<omega>) \<turnstile> \<langle>e_b; \<omega>\<rangle> [\<Down>]\<^sub>t Val (VBool True) \<rbrakk> \<Longrightarrow> 
-      red_stmt_total_single_set ctxt R \<Lambda> (If e_b s1 s2) \<omega> (Inl s1, RNormal \<omega>)"
+      red_stmt_total ctxt R \<Lambda> (If e_b s1 s2) \<omega> (RNormal \<omega>)"
  | RedIfFalse: 
    "\<lbrakk> ctxt, R, (Some \<omega>) \<turnstile> \<langle>e_b; \<omega>\<rangle> [\<Down>]\<^sub>t Val (VBool False) \<rbrakk> \<Longrightarrow> 
-      red_stmt_total_single_set ctxt R \<Lambda> (If e_b s1 s2) \<omega> (Inl s2, RNormal \<omega>)"
+      red_stmt_total ctxt R \<Lambda> (If e_b s1 s2) \<omega> (RNormal \<omega>)"
  | RedIfFailure:
     "\<lbrakk> ctxt, R, (Some \<omega>) \<turnstile> \<langle>e_b; \<omega>\<rangle> [\<Down>]\<^sub>t VFailure \<rbrakk> \<Longrightarrow>
-       red_stmt_total_single_set ctxt R \<Lambda> (If e_b s1 s2) \<omega> (Inr (), RFailure)"
- | RedSeq1:
-   "\<lbrakk> red_stmt_total_single_set ctxt R \<Lambda> s1 \<omega> (Inl s'', r'') \<rbrakk> \<Longrightarrow>
-      red_stmt_total_single_set ctxt R \<Lambda> (Seq s1 s2) \<omega> (Inl (Seq s'' s2), r'')"
- | RedSeq2: 
-   "\<lbrakk> red_stmt_total_single_set ctxt R \<Lambda> s1 \<omega> (Inr (), r'') \<rbrakk> \<Longrightarrow>
-      red_stmt_total_single_set ctxt R \<Lambda> (Seq s1 s2) \<omega> (Inl s2, r'')"
+       red_stmt_total ctxt R \<Lambda> (If e_b s1 s2) \<omega> RFailure"
+ | RedSeq:
+   "\<lbrakk> red_stmt_total ctxt R \<Lambda> s1 \<omega> (RNormal \<omega>');
+      red_stmt_total ctxt R \<Lambda> s1 \<omega>' res \<rbrakk> \<Longrightarrow>
+      red_stmt_total ctxt R \<Lambda> (Seq s1 s2) \<omega> res"
 
 \<comment>\<open>Failure subexpression\<close>
 | RedSubExpressionFailure: 
   "\<lbrakk> e \<in> sub_expressions s; ctxt, R, (Some \<omega>) \<turnstile> \<langle>e; \<omega>\<rangle> [\<Down>]\<^sub>t VFailure  \<rbrakk> \<Longrightarrow> 
-    red_stmt_total_single_set ctxt R \<Lambda> s \<omega> (Inr (), RFailure)"
+    red_stmt_total ctxt R \<Lambda> s \<omega> RFailure"
 
 inductive_cases RedLocalAssign_case: 
-     "red_stmt_total_single_set ctxt R \<Lambda> (LocalAssign x e) \<omega> (Inr (), (RNormal (update_var_total \<omega> x v)))"
-
-type_synonym 'a stmt_config = "(stmt + unit) \<times> 'a standard_result"
-
-inductive red_stmt_total_single :: "'a total_context \<Rightarrow> ('a full_total_state \<Rightarrow> bool) \<Rightarrow> type_context \<Rightarrow> 'a stmt_config \<Rightarrow> 'a stmt_config \<Rightarrow> bool"
-  where 
-    NormalSingleStep: "\<lbrakk> red_stmt_total_single_set ctxt R \<Lambda> s \<omega> res \<rbrakk> \<Longrightarrow> 
-       red_stmt_total_single ctxt R \<Lambda> ((Inl s, RNormal \<omega>)) res"
-
-inductive_cases NormalSingleStep_case [elim]: "red_stmt_total_single ctxt R \<Lambda> ((Inl s, RNormal \<omega>)) res"
-
-abbreviation red_stmt_total_multi :: "'a total_context \<Rightarrow> ('a full_total_state \<Rightarrow> bool) \<Rightarrow> type_context \<Rightarrow> 'a stmt_config \<Rightarrow> 'a stmt_config \<Rightarrow> bool"
-  where "red_stmt_total_multi ctxt R \<Lambda> \<equiv> rtranclp (red_stmt_total_single ctxt R \<Lambda>)"
+     "red_stmt_total ctxt R \<Lambda> (LocalAssign x e) \<omega> (RNormal (update_var_total \<omega> x v))"
 
 definition is_empty_total :: "'a full_total_state \<Rightarrow> bool"
   where "is_empty_total \<omega> \<equiv> get_m_total_full \<omega> = (zero_mask, zero_mask)"
-
-fun is_failure_config :: "'a stmt_config \<Rightarrow> bool"
-  where "is_failure_config config \<longleftrightarrow> (snd config) = RFailure"
-
-fun is_normal_config :: "'a stmt_config \<Rightarrow> 'a full_total_state \<Rightarrow> bool"
-  where "is_normal_config config \<omega> \<longleftrightarrow> (snd config) = RNormal \<omega>"
 
 subsection \<open>Correctness\<close>
 
@@ -280,7 +262,7 @@ definition vals_well_typed :: "('a \<Rightarrow> abs_type) \<Rightarrow> ('a val
 
 definition assertion_sat :: "'a total_context \<Rightarrow> ('a full_total_state \<Rightarrow> bool) \<Rightarrow> type_context \<Rightarrow> assertion \<Rightarrow> 'a full_total_state \<Rightarrow> bool"
   where "assertion_sat \<Lambda> R ctxt A \<omega> = 
-            (\<forall> res. red_stmt_total_single_set \<Lambda> R ctxt (Assert A) \<omega> res \<longrightarrow> (snd res) \<noteq> RFailure)"
+            (\<forall> res. red_stmt_total \<Lambda> R ctxt (Assert A) \<omega> res \<longrightarrow> res \<noteq> RFailure)"
 
 text \<open>Note that \<^const>\<open>assertion_sat\<close> is ``demonic'', i.e., every reduction of asserting \<^term>\<open>A\<close> must
 be a non-failing state, which is in-sync with the semantics of assert statements in programs. We might
@@ -340,6 +322,6 @@ definition stmt_correct_total :: " 'a total_context \<Rightarrow> ('a full_total
            heap_dep_fun_obligations ctxt R \<Lambda> \<and>
            predicate_obligations ctxt \<and>
            (\<forall>(\<omega> :: 'a full_total_state) r. is_empty_total \<omega> \<longrightarrow> 
-                red_stmt_total_multi ctxt R \<Lambda> ((Inl s, RNormal \<omega>)) r \<longrightarrow> \<not>is_failure_config r)"
+                red_stmt_total ctxt R \<Lambda> s \<omega> r \<longrightarrow> r \<noteq> RFailure)"
 
 end
